minor refactoring for remote and parallel defs

src/Axioms_Io.v
@@ -14,57 +14,66 @@ Import ListNotations.
 Definition toRemote (t:AnnoTerm) (pTo:Plc) (e:EvC) : EvC.
 Admitted.
 
-Definition remote_events (t:AnnoTerm) (p:Plc) : list Ev.
+Definition parallel_vm_thread (l:Loc) (t:AnnoTerm) (p:Plc) (e:EvC) : EvC.
 Admitted.
 
-Definition parallel_vm_thread (t:AnnoTerm) (p:Plc) (e:EvC) : EvC.
-Admitted.
-
+(*
 Definition parallel_vm_events (t:AnnoTerm) (p:Plc) : list Ev.
 Admitted.
+*)
 
 Definition shuffled_events (el1:list Ev) (el2:list Ev) : list Ev.
 Admitted.
 
-Definition remote_evidence (t:AnnoTerm) (p:Plc) (e:EvC) : EvC.
+Definition cvm_events (t:AnnoTerm) (p:Plc) (e:Evidence) : list Ev.
 Admitted.
 
+Definition cvm_evidence (t:AnnoTerm) (p:Plc) (e:EvC) : EvC.
+Admitted.
+
+(*
 Definition remote_trace (t:AnnoTerm) (p:Plc) : list Ev.
 Admitted.
+*)
 
 Axiom remote_LTS: forall t n et, 
-    lstar (conf t n et) (remote_events t n) (stop n (aeval t n et)).
+    lstar (conf t n et) (cvm_events t n et) (stop n (aeval t n et)).
 
 
+(*
 Axiom remote_Evidence_Type_Axiom: forall t n bits et,
     get_et (toRemote t n (evc bits et)) = aeval t n et.
+*)
 
 
 Axiom at_evidence : forall t (p:Plc) (e:EvC),
-    toRemote t p e = remote_evidence t p e.
+    toRemote t p e = cvm_evidence t p e.
 
+(*
 Axiom at_events : forall t p,
   remote_events t p = remote_trace t p.
+*)
 
 
-Axiom par_evidence : forall t (p:Plc) (e:EvC),
-    parallel_vm_thread t p e = remote_evidence t p e.
+Axiom par_evidence : forall t (p:Plc) (e:EvC) loc,
+    parallel_vm_thread loc t p e = cvm_evidence t p e.
 
-
+(*
 Axiom par_events : forall t p,
     parallel_vm_events t p = remote_trace t p.
+*)
 
 Axiom bpar_shuffle : forall x tr p t1 t2 et1 et2,
     lstar (conf t1 p et1) tr (stop p (aeval t1 p et1)) ->
     lstar (bp x (conf t1 p et1) (conf t2 p et2))
           (shuffled_events tr
-                           (remote_events t2 p))
+                           (cvm_events t2 p et2))
           (bp x (stop p (aeval t1 p et1)) (stop p (aeval t2 p et2))).
 
-Axiom thread_bookend_peel: forall t p et etr n l a n0 tr,
-    lstar (conf (unannoPar t) p et) tr (stop p (aeval (unannoPar t) p et)) ->
-    ([cvm_thread_start n l p a etr] ++ tr ++ [cvm_thread_end (Nat.pred n0) l p a] =
-     (shuffled_events tr (remote_events a p))
+Axiom thread_bookend_peel: forall t p et etr l a tr,
+    lstar (conf t p et) tr (stop p (aeval t p et)) ->
+    ([cvm_thread_start l p a etr] ++ tr ++ [cvm_thread_end l] =
+     (shuffled_events tr (cvm_events a p etr))
     ).
 
 Axiom wf_ec_preserved_remote: forall a n e,
